proof/Verif_u128_from_u64.v
@@ -1,0 +1,47 @@
+(** * Verif_u128_from_u64: Proof of body_secp256k1_u128_from_u64 *)
+(** Copyright (C) 2026 remix7531
+    SPDX-License-Identifier: GPL-3.0-or-later *)
+
+Require Import scalar_4x64.Verif_imports.
+Require Import scalar_4x64.Helper_verif.
+
+(* ================================================================= *)
+(** ** secp256k1_u128_from_u64 *)
+
+Lemma u64_lt_u128 (a : UInt64) : 0 <= u64_val a < 2^128.
+Proof.
+  destruct a.
+  simpl.
+  lia.
+Qed.
+
+Lemma u64_uint128_repr (a : UInt64) :
+  uint128_to_val (mkUInt128 (u64_val a) (u64_lt_u128 a)) =
+  (uint64_to_val a, Vlong (Int64.repr 0)).
+Proof.
+  unfold uint128_to_val, uint64_to_val, limb64.
+  simpl Z.of_nat.
+  simpl Z.mul.
+  simpl u128_val.
+  simpl Z.pow.
+  rewrite Z.div_1_r.
+  pose proof (u64_range a) as Ha.
+  do 4 f_equal.
+  - apply Z.mod_small; lia.
+  - rewrite Z.div_small by lia.
+    reflexivity.
+Qed.
+
+Lemma body_secp256k1_u128_from_u64:
+  semax_body Vprog Gprog
+    f_secp256k1_u128_from_u64 secp256k1_u128_from_u64_spec.
+Proof.
+  start_function.
+
+  forward. (* r->lo = a *)
+  forward. (* r->hi = 0 *)
+
+  Exists (mkUInt128 (u64_val a) (u64_lt_u128 a)).
+  rewrite u64_uint128_repr.
+  entailer!.
+Qed.
