proof/Verif_u128_mul.v
@@ -1,0 +1,41 @@
+(** * Verif_u128_mul: Proof of body_secp256k1_u128_mul *)
+(** Copyright (C) 2026 remix7531
+    SPDX-License-Identifier: GPL-3.0-or-later *)
+
+Require Import scalar_4x64.Verif_imports.
+Require Import scalar_4x64.Helper_verif.
+
+(* ================================================================= *)
+(** ** secp256k1_u128_mul *)
+
+(** Plumbing around the umul128 spec. *)
+
+Lemma body_secp256k1_u128_mul:
+  semax_body Vprog Gprog
+    f_secp256k1_u128_mul secp256k1_u128_mul_spec.
+Proof.
+  start_function.
+
+  (* Decompose uninitialised struct into .lo and .hi fields *)
+  unfold data_at_, field_at_.
+  unfold_data_at (field_at sh t_secp256k1_uint128 [] _ r_ptr).
+  assert_PROP (field_compatible t_secp256k1_uint128 [StructField _hi] r_ptr)
+    as Hfc by entailer!.
+  rewrite (field_at_data_at sh _ [StructField _hi]) by reflexivity.
+
+  (* r->lo = secp256k1_umul128(a, b, &r->hi) *)
+  forward_call (a, b,
+    field_address t_secp256k1_uint128 [StructField _hi] r_ptr, sh).
+  Intros vret.
+
+  (* r->lo = _t'1 *)
+  forward.
+
+  (* Provide witness and reassemble struct *)
+  Exists vret.
+  entailer!.
+  unfold uint128_to_val.
+  unfold_data_at (data_at sh t_secp256k1_uint128 _ r_ptr).
+  rewrite (field_at_data_at sh _ [StructField _hi]) by reflexivity.
+  cancel.
+Qed.
